theories/typing.v
@@ -16,13 +16,21 @@ Arguments module_ctx : clear implicits.
 
 Definition local_ctx := list type.
 
+Record kind_ctx :=
+  { kc_mem_vars : nat;
+    kc_rep_vars : nat;
+    kc_size_vars : nat }.
+
+Definition kc_empty : kind_ctx :=
+  {| kc_mem_vars := 0;
+     kc_rep_vars := 0;
+     kc_size_vars := 0 |}.
+
 Record function_ctx :=
   { fc_return : list type;
     fc_locals : list representation;
     fc_labels : list (list type * local_ctx);
-    fc_mem_vars : nat;
-    fc_rep_vars : nat;
-    fc_size_vars : nat;
+    fc_kind_ctx : kind_ctx;
     fc_type_vars : list kind }.
 
 Arguments function_ctx : clear implicits.
@@ -31,9 +39,7 @@ Definition fc_empty : function_ctx :=
   {| fc_return := [];
      fc_locals := [];
      fc_labels := [];
-     fc_mem_vars := 0;
-     fc_rep_vars := 0;
-     fc_size_vars := 0;
+     fc_kind_ctx := kc_empty;
      fc_type_vars := [] |}.
 
 Definition subst_function_ctx
@@ -47,134 +53,132 @@ Definition subst_function_ctx
          (fun '(τs, L) =>
             (map (subst_type s__mem s__rep s__size s__type) τs, map (subst_type s__mem s__rep s__size s__type) L))
          F.(fc_labels);
-     fc_mem_vars := F.(fc_mem_vars);
-     fc_rep_vars := F.(fc_rep_vars);
-     fc_size_vars := F.(fc_size_vars);
+     fc_kind_ctx := F.(fc_kind_ctx);
      fc_type_vars := map (subst_kind s__mem s__rep s__size) F.(fc_type_vars) |}.
 
 Global Instance eta_function_ctx : Settable _ :=
   settable! Build_function_ctx
-  <fc_return; fc_locals; fc_labels; fc_mem_vars; fc_rep_vars; fc_size_vars; fc_type_vars>.
+  <fc_return; fc_locals; fc_labels; fc_kind_ctx; fc_type_vars>.
 
 Definition update_locals (ξ : local_fx) (L : local_ctx) : local_ctx :=
   let 'LocalFx l := ξ in
   fold_left (fun acc '(i, τ) => <[ i := τ ]> acc) l L.
 
-Inductive mem_ok : function_ctx -> memory -> Prop :=
-| OKVarM F m :
-  m < F.(fc_mem_vars) ->
-  mem_ok F (VarM m)
-| OKConstM F cm :
-  mem_ok F (ConstM cm).
+Inductive mem_ok : kind_ctx -> memory -> Prop :=
+| OKVarM K m :
+  m < K.(kc_mem_vars) ->
+  mem_ok K (VarM m)
+| OKConstM K cm :
+  mem_ok K (ConstM cm).
 
-Inductive rep_ok : function_ctx -> representation -> Prop :=
-| OKVarR F r :
-  r < F.(fc_rep_vars) ->
-  rep_ok F (VarR r)
-| OKSumR F ρs :
-  Forall (rep_ok F) ρs ->
-  rep_ok F (SumR ρs)
-| OKProdR F ρs :
-  Forall (rep_ok F) ρs ->
-  rep_ok F (ProdR ρs)
-| OKPrimR F ι :
-  rep_ok F (PrimR ι).
+Inductive rep_ok : kind_ctx -> representation -> Prop :=
+| OKVarR K r :
+  r < K.(kc_rep_vars) ->
+  rep_ok K (VarR r)
+| OKSumR K ρs :
+  Forall (rep_ok K) ρs ->
+  rep_ok K (SumR ρs)
+| OKProdR K ρs :
+  Forall (rep_ok K) ρs ->
+  rep_ok K (ProdR ρs)
+| OKPrimR K ι :
+  rep_ok K (PrimR ι).
 
-Inductive size_ok : function_ctx -> size -> Prop :=
-| OKVarS F s :
-  s < F.(fc_size_vars) ->
-  size_ok F (VarS s)
-| OKSumS F σs :
-  Forall (size_ok F) σs ->
-  size_ok F (SumS σs)
-| OKProdS F σs :
-  Forall (size_ok F) σs ->
-  size_ok F (ProdS σs)
-| OKRepS F ρ :
-  rep_ok F ρ ->
-  size_ok F (RepS ρ)
-| OKConstS F n :
-  size_ok F (ConstS n).
+Inductive size_ok : kind_ctx -> size -> Prop :=
+| OKVarS K s :
+  s < K.(kc_size_vars) ->
+  size_ok K (VarS s)
+| OKSumS K σs :
+  Forall (size_ok K) σs ->
+  size_ok K (SumS σs)
+| OKProdS K σs :
+  Forall (size_ok K) σs ->
+  size_ok K (ProdS σs)
+| OKRepS K ρ :
+  rep_ok K ρ ->
+  size_ok K (RepS ρ)
+| OKConstS K n :
+  size_ok K (ConstS n).
 
-Inductive sizity_ok : function_ctx -> sizity -> Prop :=
-| OKSized F σ :
-  size_ok F σ ->
-  sizity_ok F (Sized σ)
-| OKUnsized F :
-  sizity_ok F Unsized.
+Inductive sizity_ok : kind_ctx -> sizity -> Prop :=
+| OKSized K σ :
+  size_ok K σ ->
+  sizity_ok K (Sized σ)
+| OKUnsized K :
+  sizity_ok K Unsized.
 
-Inductive kind_ok : function_ctx -> kind -> Prop :=
-| OKVALTYPE (F : function_ctx) (ρ : representation) (χ : copyability) (δ : dropability) :
-  rep_ok F ρ ->
-  kind_ok F (VALTYPE ρ χ δ)
-| OKMEMTYPE (F : function_ctx) (ζ : sizity) (μ : memory) (δ : dropability) :
-  sizity_ok F ζ ->
-  mem_ok F μ ->
-  kind_ok F (MEMTYPE ζ μ δ).
+Inductive kind_ok : kind_ctx -> kind -> Prop :=
+| OKVALTYPE K ρ χ δ :
+  rep_ok K ρ ->
+  kind_ok K (VALTYPE ρ χ δ)
+| OKMEMTYPE K ζ μ δ :
+  sizity_ok K ζ ->
+  mem_ok K μ ->
+  kind_ok K (MEMTYPE ζ μ δ).
 
 Inductive type_ok : function_ctx -> type -> Prop :=
 | OKVarT F t κ :
   F.(fc_type_vars) !! t = Some κ ->
-  kind_ok F κ ->
+  kind_ok F.(fc_kind_ctx) κ ->
   type_ok F (VarT t)
 | OKNumT F κ ν :
-  kind_ok F κ ->
+  kind_ok F.(fc_kind_ctx) κ ->
   type_ok F (NumT κ ν)
 | OKSumT F κ τs :
-  kind_ok F κ ->
+  kind_ok F.(fc_kind_ctx) κ ->
   Forall (type_ok F) τs ->
   type_ok F (SumT κ τs)
 | OKProdT F κ τs :
-  kind_ok F κ ->
+  kind_ok F.(fc_kind_ctx) κ ->
   Forall (type_ok F) τs ->
   type_ok F (ProdT κ τs)
 | OKRefT F κ μ τ :
-  kind_ok F κ ->
-  mem_ok F μ ->
+  kind_ok F.(fc_kind_ctx) κ ->
+  mem_ok F.(fc_kind_ctx) μ ->
   type_ok F τ ->
   type_ok F (RefT κ μ τ)
 | OKGCPtr F κ τ :
-  kind_ok F κ ->
+  kind_ok F.(fc_kind_ctx) κ ->
   type_ok F τ ->
   type_ok F (GCPtrT κ τ)
 | OKCodeRefT F κ ϕ :
-  kind_ok F κ ->
+  kind_ok F.(fc_kind_ctx) κ ->
   function_type_ok F ϕ ->
   type_ok F (CodeRefT κ ϕ)
 | OKRepT F κ ρ τ :
-  kind_ok F κ ->
-  rep_ok F ρ ->
+  kind_ok F.(fc_kind_ctx) κ ->
+  rep_ok F.(fc_kind_ctx) ρ ->
   type_ok F τ ->
   type_ok F (RepT κ ρ τ)
 | OKPadT F κ σ τ :
-  kind_ok F κ ->
-  size_ok F σ ->
+  kind_ok F.(fc_kind_ctx) κ ->
+  size_ok F.(fc_kind_ctx) σ ->
   type_ok F τ ->
   type_ok F (PadT κ σ τ)
 | OKSerT F κ τ :
-  kind_ok F κ ->
+  kind_ok F.(fc_kind_ctx) κ ->
   type_ok F τ ->
   type_ok F (SerT κ τ)
 | OKRecT F κ τ :
-  kind_ok F κ ->
-  type_ok F τ ->
+  kind_ok F.(fc_kind_ctx) κ ->
+  type_ok (F <| fc_type_vars ::= cons κ |>) τ ->
   type_ok F (RecT κ τ)
 | OKExistsMemT F κ τ :
-  kind_ok F κ ->
-  type_ok (set fc_mem_vars S F) τ ->
+  kind_ok F.(fc_kind_ctx) κ ->
+  type_ok (F <| fc_kind_ctx ::= set kc_mem_vars S |>) τ ->
   type_ok F (ExistsMemT κ τ)
 | OKExistsRepT F κ τ :
-  kind_ok F κ ->
-  type_ok (set fc_rep_vars S F) τ ->
+  kind_ok F.(fc_kind_ctx) κ ->
+  type_ok (F <| fc_kind_ctx ::= set kc_rep_vars S |>) τ ->
   type_ok F (ExistsRepT κ τ)
 | OKExistsSizeT F κ τ :
-  kind_ok F κ ->
-  type_ok (set fc_size_vars S F) τ ->
+  kind_ok F.(fc_kind_ctx) κ ->
+  type_ok (F <| fc_kind_ctx ::= set kc_size_vars S |>) τ ->
   type_ok F (ExistsSizeT κ τ)
 | OKExistsType F κ κ0 τ :
-  kind_ok F κ ->
-  kind_ok F κ0 ->
-  type_ok (set fc_type_vars (cons κ0) F) τ ->
+  kind_ok F.(fc_kind_ctx) κ ->
+  kind_ok F.(fc_kind_ctx) κ0 ->
+  type_ok (F <| fc_type_vars ::= cons κ0 |>) τ ->
   type_ok F (ExistsTypeT κ κ0 τ)
 
 with instruction_type_ok : function_ctx -> instruction_type -> Prop :=
@@ -188,17 +192,17 @@ with function_type_ok : function_ctx -> function_type -> Prop :=
   instruction_type_ok F ψ ->
   function_type_ok F (MonoFunT ψ)
 | OKForallMemT F ϕ :
-  function_type_ok (set fc_mem_vars S F) ϕ ->
+  function_type_ok (F <| fc_kind_ctx ::= set kc_mem_vars S |>) ϕ ->
   function_type_ok F (ForallMemT ϕ)
 | OKForallRepT F ϕ :
-  function_type_ok (set fc_rep_vars S F) ϕ ->
+  function_type_ok (F <| fc_kind_ctx ::= set kc_rep_vars S |>) ϕ ->
   function_type_ok F (ForallRepT ϕ)
 | OKForallSizeT F ϕ :
-  function_type_ok (set fc_size_vars S F) ϕ ->
+  function_type_ok (F <| fc_kind_ctx ::= set kc_size_vars S |>) ϕ ->
   function_type_ok F (ForallSizeT ϕ)
 | OKForallTypeT F κ ϕ :
-  kind_ok F κ ->
-  function_type_ok (set fc_type_vars (cons κ) F) ϕ ->
+  kind_ok F.(fc_kind_ctx) κ ->
+  function_type_ok (F <| fc_type_vars ::= cons κ |>) ϕ ->
   function_type_ok F (ForallTypeT κ ϕ).
 
 Definition mono_mem (μ : memory) : Prop :=
@@ -220,6 +224,12 @@ Inductive sub_kind : kind -> kind -> Prop :=
 | KSubSizity σ μ δ :
   sub_kind (MEMTYPE (Sized σ) μ δ) (MEMTYPE Unsized μ δ).
 
+Inductive has_kind_ok : function_ctx -> type -> kind -> Prop :=
+| OKHasKind F τ κ :
+  type_ok F τ ->
+  kind_ok F.(fc_kind_ctx) κ ->
+  has_kind_ok F τ κ.
+
 Inductive has_kind : function_ctx -> type -> kind -> Prop :=
 | KSub F τ κ κ' :
   sub_kind κ κ' ->
@@ -227,7 +237,7 @@ Inductive has_kind : function_ctx -> type -> kind -> Prop :=
   has_kind F τ κ'
 | KVar F t κ :
   F.(fc_type_vars) !! t = Some κ ->
-  kind_ok F κ ->
+  kind_ok F.(fc_kind_ctx) κ ->
   has_kind F (VarT t) κ
 | KI32 F :
   let κ := VALTYPE (PrimR I32R) ImCopy ImDrop in
@@ -246,10 +256,12 @@ Inductive has_kind : function_ctx -> type -> kind -> Prop :=
   let κ := VALTYPE (SumR ρs) χ δ in
   has_kind F (SumT κ τs) κ
 | KSumMem F τs ζs μ δ :
+  mem_ok F.(fc_kind_ctx) μ ->
   Forall2 (fun τ ζ => has_kind F τ (MEMTYPE ζ μ δ)) τs ζs ->
   let κ := MEMTYPE Unsized μ δ in
   has_kind F (SumT κ τs) κ
 | KSumMemSized F τs σs μ δ :
+  mem_ok F.(fc_kind_ctx) μ ->
   Forall2 (fun τ σ => has_kind F τ (MEMTYPE (Sized σ) μ δ)) τs σs ->
   let κ := MEMTYPE (Sized (SumS σs)) μ δ in
   has_kind F (SumT κ τs) κ
@@ -258,14 +270,16 @@ Inductive has_kind : function_ctx -> type -> kind -> Prop :=
   let κ := VALTYPE (ProdR ρs) χ δ in
   has_kind F (ProdT κ τs) κ
 | KProdMem F τs ζs μ δ :
+  mem_ok F.(fc_kind_ctx) μ ->
   Forall2 (fun τ ζ => has_kind F τ (MEMTYPE ζ μ δ)) τs ζs ->
   let κ := MEMTYPE Unsized μ δ in
   has_kind F (ProdT κ τs) κ
 | KProdMemSized F τs σs μ δ :
+  mem_ok F.(fc_kind_ctx) μ ->
   Forall2 (fun τ σ => has_kind F τ (MEMTYPE (Sized σ) μ δ)) τs σs ->
   let κ := MEMTYPE (Sized (ProdS σs)) μ δ in
   has_kind F (ProdT κ τs) κ
-| KRef F (μ : memory) τ ζ μ δ :
+| KRef F τ ζ μ δ :
   has_kind F τ (MEMTYPE ζ μ δ) ->
   let κ := VALTYPE (PrimR PtrR) NoCopy NoDrop in
   has_kind F (RefT κ μ τ) κ
@@ -282,36 +296,162 @@ Inductive has_kind : function_ctx -> type -> kind -> Prop :=
   let κ := MEMTYPE (Sized (ConstS 1)) (ConstM MemGC) ImDrop in
   has_kind F (GCPtrT κ τ) κ
 | KCodeRef F ϕ :
+  function_type_ok F ϕ ->
   let κ := VALTYPE (PrimR I32R) ImCopy ImDrop in
   has_kind F (CodeRefT κ ϕ) κ
 | KRep F ρ0 ρ τ χ δ :
   has_kind F τ (VALTYPE ρ0 χ δ) ->
+  rep_ok F.(fc_kind_ctx) ρ ->
   let κ := VALTYPE ρ χ δ in
   has_kind F (RepT κ ρ τ) κ
 | KPad F σ0 σ τ μ δ :
   has_kind F τ (MEMTYPE (Sized σ0) μ δ) ->
+  size_ok F.(fc_kind_ctx) σ ->
   let κ := MEMTYPE (Sized σ) μ δ in
   has_kind F (PadT κ σ τ) κ
 | KSer F τ ρ μ χ δ :
+  mem_ok F.(fc_kind_ctx) μ ->
   has_kind F τ (VALTYPE ρ χ δ) ->
   let κ := MEMTYPE (Sized (RepS ρ)) μ δ in
   has_kind F (SerT κ τ) κ
 | KRec F τ κ :
-  let τ0 := subst_type VarM VarR VarS (unscoped.scons (RecT κ τ) VarT) τ in
-  has_kind F τ0 κ ->
+  has_kind (F <| fc_type_vars ::= cons κ |>) τ κ ->
   has_kind F (RecT κ τ) κ
 | KExistsMem F τ κ :
-  has_kind (set fc_mem_vars S F) τ κ ->
+  has_kind (F <| fc_kind_ctx ::= set kc_mem_vars S |>) τ κ ->
+  kind_ok F.(fc_kind_ctx) κ ->
   has_kind F (ExistsMemT κ τ) κ
 | KExistsRep F τ κ :
-  has_kind (set fc_rep_vars S F) τ κ ->
+  has_kind (F <| fc_kind_ctx ::= set kc_rep_vars S |>) τ κ ->
+  kind_ok F.(fc_kind_ctx) κ ->
   has_kind F (ExistsRepT κ τ) κ
 | KExistsSize F τ κ :
-  has_kind (set fc_size_vars S F) τ κ ->
+  has_kind (F <| fc_kind_ctx ::= set kc_size_vars S |>) τ κ ->
+  kind_ok F.(fc_kind_ctx) κ ->
   has_kind F (ExistsSizeT κ τ) κ
 | KExistsType F τ κ0 κ :
-  has_kind (set fc_type_vars (cons κ0) F) τ κ ->
+  kind_ok F.(fc_kind_ctx) κ0 ->
+  kind_ok F.(fc_kind_ctx) κ ->
+  has_kind (F <| fc_type_vars ::= cons κ0 |>) τ κ ->
   has_kind F (ExistsTypeT κ κ0 τ) κ.
+
+Section HasKindInd.
+
+  Variable P : function_ctx -> type -> kind -> Prop.
+
+  Hypotheses
+    (HSub : forall F τ κ κ', sub_kind κ κ' -> P F τ κ -> P F τ κ')
+      (HVar : forall F t κ, F.(fc_type_vars) !! t = Some κ ->
+                       kind_ok F.(fc_kind_ctx) κ ->
+                       P F (VarT t) κ)
+      (HI32 : forall F, let κ := VALTYPE (PrimR I32R) ImCopy ImDrop in
+                   P F (NumT κ (IntT I32T)) κ)
+      (HI64 : forall F, let κ := VALTYPE (PrimR I64R) ImCopy ImDrop in
+                   P F (NumT κ (IntT I64T)) κ)
+      (HF32 : forall F, let κ := VALTYPE (PrimR F32R) ImCopy ImDrop in
+                   P F (NumT κ (FloatT F32T)) κ)
+      (HF64 : forall F, let κ := VALTYPE (PrimR F64R) ImCopy ImDrop in
+                   P F (NumT κ (FloatT F64T)) κ)
+      (HSumVal : forall F τs ρs χ δ, Forall2 (fun τ ρ => P F τ (VALTYPE ρ χ δ)) τs ρs ->
+                                let κ := VALTYPE (SumR ρs) χ δ in
+                                P F (SumT κ τs) κ)
+      (HSumMem : forall F τs ζs μ δ, mem_ok F.(fc_kind_ctx) μ ->
+                                Forall2 (fun τ ζ => P F τ (MEMTYPE ζ μ δ)) τs ζs ->
+                                let κ := MEMTYPE Unsized μ δ in P F (SumT κ τs) κ)
+      (HSumMemSized : forall F τs σs μ δ,
+          mem_ok F.(fc_kind_ctx) μ ->
+          Forall2 (fun τ σ => P F τ (MEMTYPE (Sized σ) μ δ)) τs σs ->
+          let κ := MEMTYPE (Sized (SumS σs)) μ δ in P F (SumT κ τs) κ)
+      (HProdVal : forall F τs ρs χ δ, Forall2 (fun τ ρ => P F τ (VALTYPE ρ χ δ)) τs ρs ->
+                                 let κ := VALTYPE (ProdR ρs) χ δ in
+                                 P F (ProdT κ τs) κ)
+      (HProdMem : forall F τs ζs μ δ, mem_ok F.(fc_kind_ctx) μ ->
+                                 Forall2 (fun τ ζ => P F τ (MEMTYPE ζ μ δ)) τs ζs ->
+                                 let κ := MEMTYPE Unsized μ δ in
+                                 P F (ProdT κ τs) κ)
+      (HProdMemSized : forall F τs σs μ δ, mem_ok F.(fc_kind_ctx) μ ->
+                                      Forall2 (fun τ σ => P F τ (MEMTYPE (Sized σ) μ δ)) τs σs ->
+                                      let κ := MEMTYPE (Sized (ProdS σs)) μ δ in
+                                      P F (ProdT κ τs) κ)
+      (HRef : forall F τ ζ μ δ, P F τ (MEMTYPE ζ μ δ) ->
+                           let κ := VALTYPE (PrimR PtrR) NoCopy NoDrop in
+                           P F (RefT κ μ τ) κ)
+      (HRefMMDrop : forall F τ ζ, P F τ (MEMTYPE ζ (ConstM MemMM) ImDrop) ->
+                             let κ := VALTYPE (PrimR PtrR) NoCopy ExDrop in
+                             P F (RefT κ (ConstM MemMM) τ) κ)
+      (HRefGC : forall F τ ζ δ, P F τ (MEMTYPE ζ (ConstM MemGC) δ) ->
+                           let κ := VALTYPE (PrimR PtrR) ExCopy ExDrop in
+                           P F (RefT κ (ConstM MemGC) τ) κ)
+      (HGCPtr : forall F τ ζ δ, P F τ (MEMTYPE ζ (ConstM MemGC) δ) ->
+                           let κ := MEMTYPE (Sized (ConstS 1)) (ConstM MemGC) ImDrop in
+                           P F (GCPtrT κ τ) κ)
+      (HCodeRef : forall F ϕ, function_type_ok F ϕ ->
+                         let κ := VALTYPE (PrimR I32R) ImCopy ImDrop in
+                         P F (CodeRefT κ ϕ) κ)
+      (HRep : forall F ρ0 ρ τ χ δ, P F τ (VALTYPE ρ0 χ δ) ->
+                              rep_ok F.(fc_kind_ctx) ρ ->
+                              let κ := VALTYPE ρ χ δ in
+                              P F (RepT κ ρ τ) κ)
+      (HPad : forall F σ0 σ τ μ δ, P F τ (MEMTYPE (Sized σ0) μ δ) ->
+                              size_ok F.(fc_kind_ctx) σ ->
+                              let κ := MEMTYPE (Sized σ) μ δ in
+                              P F (PadT κ σ τ) κ)
+      (HSer : forall F τ ρ μ χ δ, mem_ok F.(fc_kind_ctx) μ ->
+                             P F τ (VALTYPE ρ χ δ) ->
+                             let κ := MEMTYPE (Sized (RepS ρ)) μ δ in
+                             P F (SerT κ τ) κ)
+      (HRec : forall F τ κ, P (F <| fc_type_vars ::= cons κ |>) τ κ ->
+                       P F (RecT κ τ) κ)
+      (HExistsMem : forall F τ κ, P (F <| fc_kind_ctx ::= set kc_mem_vars S |>) τ κ ->
+                             kind_ok F.(fc_kind_ctx) κ ->
+                             P F (ExistsMemT κ τ) κ)
+      (HExistsRep : forall F τ κ, P (F <| fc_kind_ctx ::= set kc_rep_vars S |>) τ κ ->
+                             kind_ok F.(fc_kind_ctx) κ ->
+                             P F (ExistsRepT κ τ) κ)
+      (HExistsSize : forall F τ κ, P (F <| fc_kind_ctx ::= set kc_size_vars S |>) τ κ ->
+                              kind_ok F.(fc_kind_ctx) κ ->
+                              P F (ExistsSizeT κ τ) κ)
+      (HExistsType : forall F τ κ0 κ, kind_ok F.(fc_kind_ctx) κ0 ->
+                                 kind_ok F.(fc_kind_ctx) κ ->
+                                 P (F <| fc_type_vars ::= cons κ0 |>) τ κ ->
+                                 P F (ExistsTypeT κ κ0 τ) κ).
+
+  Fixpoint has_kind_ind' (F : function_ctx) (τ : type) (κ : kind) (H : has_kind F τ κ) : P F τ κ :=
+    match H with
+    | KSub F τ κ κ' H1 H2 => HSub F τ κ κ' H1 (has_kind_ind' F τ κ H2)
+    | KVar F t κ H1 H2 => HVar F t κ H1 H2
+    | KI32 F => HI32 F
+    | KI64 F => HI64 F
+    | KF32 F => HF32 F
+    | KF64 F => HF64 F
+    | KSumVal F τs ρs χ δ H1 =>
+        HSumVal F τs ρs χ δ (Forall2_impl _ _ _ _ H1 (fun τ ρ => has_kind_ind' _ _ _))
+    | KSumMem F τs ζs μ δ H1 H2 =>
+        HSumMem F τs ζs μ δ H1 (Forall2_impl _ _ _ _ H2 (fun τ ζ => has_kind_ind' _ _ _))
+    | KSumMemSized F τs σs μ δ H1 H2 =>
+        HSumMemSized F τs σs μ δ H1 (Forall2_impl _ _ _ _ H2 (fun τ σ => has_kind_ind' _ _ _))
+    | KProdVal F τs ρs χ δ H1 H2 =>
+        HProdVal F τs ρs χ δ (Forall2_impl _ _ _ _ H1 (fun τ ρ => has_kind_ind' _ _ _))
+    | KProdMem F τs ζs μ δ H1 H2 =>
+        HProdMem F τs ζs μ δ H1 (Forall2_impl _ _ _ _ H2 (fun τ ζ => has_kind_ind' _ _ _))
+    | KProdMemSized F τs σs μ δ H1 H2 =>
+        HProdMemSized F τs σs μ δ H1 (Forall2_impl _ _ _ _ H2 (fun τ σ => has_kind_ind' _ _ _))
+    | KRef F τ ζ μ δ H1 => HRef F τ ζ μ δ (has_kind_ind' _ _ _ H1)
+    | KRefMMDrop F τ ζ H1 => HRefMMDrop F τ ζ (has_kind_ind' _ _ _ H1)
+    | KRefGC F τ ζ δ H1 => HRefGC F τ ζ δ (has_kind_ind' _ _ _ H1)
+    | KGCPtr F τ ζ δ H1 => HGCPtr F τ ζ δ (has_kind_ind' _ _ _ H1)
+    | KCodeRef F ϕ H1 => HCodeRef F ϕ H1
+    | KRep F ρ0 ρ τ χ δ H1 H2 => HRep F ρ0 ρ τ χ δ (has_kind_ind' _ _ _ H1) H2
+    | KPad F σ0 σ τ μ δ H1 H2 => HPad F σ0 σ τ μ δ (has_kind_ind' _ _ _ H1) H2
+    | KSer F τ ρ μ χ δ H1 H2 => HSer F τ ρ μ χ δ H1 (has_kind_ind' _ _ _ H2)
+    | KRec F τ κ H1 => HRec F τ κ (has_kind_ind' _ _ _ H1)
+    | KExistsMem F τ κ H1 H2 => HExistsMem F τ κ (has_kind_ind' _ _ _ H1) H2
+    | KExistsRep F τ κ H1 H2 => HExistsRep F τ κ (has_kind_ind' _ _ _ H1) H2
+    | KExistsSize F τ κ H1 H2 => HExistsSize F τ κ (has_kind_ind' _ _ _ H1) H2
+    | KExistsType F τ κ0 κ H1 H2 H3 => HExistsType F τ κ0 κ H1 H2 (has_kind_ind' _ _ _ H3)
+    end.
+
+End HasKindInd.
 
 Inductive has_rep : function_ctx -> type -> representation -> Prop :=
 | RepVALTYPE F τ ρ χ δ :
@@ -430,13 +570,6 @@ Inductive stores_as : function_ctx -> type -> type -> Prop :=
 
 Definition loads_as F τ τ' := stores_as F τ' τ.
 
-Inductive module_ctx_ok : module_ctx -> Prop :=
-| OKModuleCtx fs ts gs :
-  Forall (function_type_ok fc_empty) fs ->
-  Forall (function_type_ok fc_empty) ts ->
-  Forall (fun '(_, τ) => type_ok fc_empty τ /\ exists ρ χ, has_kind fc_empty τ (VALTYPE ρ χ ImDrop)) gs ->
-  module_ctx_ok {| mc_functions := fs; mc_table := ts; mc_globals := gs |}.
-
 Inductive inst_function_type : function_ctx -> index -> function_type -> function_type -> Prop :=
 | FTInstMem F ϕ μ :
   let ϕ' := subst_function_type (unscoped.scons μ VarM) VarR VarS VarT ϕ in
@@ -482,13 +615,21 @@ Inductive pack_existential_type : function_ctx -> type -> type -> Prop :=
 (* TODO *)
 Inductive num_instr_has_type : num_instruction -> instruction_type -> Prop :=.
 
+Inductive has_type_ok : function_ctx -> local_ctx -> instruction_type -> local_ctx -> Prop :=
+| OKHasType F L τs1 τs2 L' :
+  Forall (type_ok F) L ->
+  Forall (type_ok F) L' ->
+  Forall (mono_rep F) τs1 ->
+  Forall (mono_rep F) τs2 ->
+  has_type_ok F L (InstrT τs1 τs2) L'.
+
 Inductive instr_has_type :
   module_ctx -> function_ctx -> local_ctx -> instruction -> instruction_type -> local_ctx -> Prop :=
 | TNop M F L :
   let ψ := InstrT [] [] in
   instr_has_type M F L (INop ψ) ψ L
-| TUnreachable M F L L' τs1 τs2 :
-  let ψ := InstrT τs1 τs2 in
+| TUnreachable M F L ψ L' :
+  has_type_ok F L ψ L' ->
   instr_has_type M F L (IUnreachable ψ) ψ L'
 | TCopy M F L τ :
   has_copyability F τ ExCopy ->
@@ -630,7 +771,8 @@ Inductive instr_has_type :
   let ψ := InstrT [τ] [τ'] in
   instr_has_type M F L (IPack ψ) ψ L
 | TUnpackMem M F L κ τ τs1 τs2 ξ es :
-  let F' := set fc_mem_vars S (subst_function_ctx (up_memory VarM) VarR VarS VarT F) in
+  let F' := subst_function_ctx (up_memory VarM) VarR VarS VarT F
+              <| fc_kind_ctx ::= set kc_mem_vars S |> in
   let L' := update_locals ξ L in
   let weak_t := map (subst_type (up_memory VarM) VarR VarS VarT) in
   let weak_e := map (subst_instruction (up_memory VarM) VarR VarS VarT) in
@@ -638,7 +780,8 @@ Inductive instr_has_type :
   let ψ := InstrT (τs1 ++ [ExistsMemT κ τ]) τs2 in
   instr_has_type M F L (IUnpack ψ ξ es) ψ L'
 | TUnpackRep M F L κ τ τs1 τs2 ξ es :
-  let F' := set fc_rep_vars S (subst_function_ctx VarM (up_representation VarR) VarS VarT F) in
+  let F' := subst_function_ctx VarM (up_representation VarR) VarS VarT F
+              <| fc_kind_ctx ::= set kc_rep_vars S |> in
   let L' := update_locals ξ L in
   let weak_t := map (subst_type VarM (up_representation VarR) VarS VarT) in
   let weak_e := map (subst_instruction VarM (up_representation VarR) VarS VarT) in
@@ -646,7 +789,8 @@ Inductive instr_has_type :
   let ψ := InstrT (τs1 ++ [ExistsRepT κ τ]) τs2 in
   instr_has_type M F L (IUnpack ψ ξ es) ψ L'
 | TUnpackSize M F L κ τ τs1 τs2 ξ es :
-  let F' := set fc_size_vars S (subst_function_ctx VarM VarR (up_size VarS) VarT F) in
+  let F' := subst_function_ctx VarM VarR (up_size VarS) VarT F
+              <| fc_kind_ctx ::= set kc_size_vars S |> in
   let L' := update_locals ξ L in
   let weak_t := map (subst_type VarM VarR (up_size VarS) VarT) in
   let weak_e := map (subst_instruction VarM VarR (up_size VarS) VarT) in
@@ -689,7 +833,7 @@ Inductive instr_has_type :
   Forall (mono_size F) pr.(pr_prefix) ->
   has_kind F pr.(pr_target) (VALTYPE ρ ImCopy δ) ->
   loads_as F pr.(pr_target) τ_val ->
-  rep_ok fc_empty ρ ->
+  rep_ok kc_empty ρ ->
   let τ_ref := RefT κ μ τ in
   has_kind F τ_ref κ ->
   let ψ := InstrT [τ_ref] [τ_ref; τ_val] in
@@ -746,3 +890,215 @@ with instrs_have_type :
 
 Scheme instr_has_type_mind := Induction for instr_has_type Sort Prop
 with instrs_have_type_mind := Induction for instrs_have_type Sort Prop.
+
+Lemma sub_kind_kind_ok F κ κ' : kind_ok F κ -> sub_kind κ κ' -> kind_ok F κ'.
+Proof.
+  intros Hk Hs.
+  induction Hs; repeat constructor; by inversion Hk.
+Qed.
+
+Lemma has_kind_inv F τ κ : has_kind F τ κ -> has_kind_ok F τ κ.
+Proof.
+  intros H.
+  induction H using has_kind_ind'.
+  - destruct IHhas_kind.
+    apply (sub_kind_kind_ok _ _ _ H1) in H.
+    split; assumption.
+  - split.
+    + eapply OKVarT.
+      * exact H.
+      * assumption.
+    + assumption.
+  - repeat constructor.
+  - repeat constructor.
+  - repeat constructor.
+  - repeat constructor.
+  - split.
+    + constructor.
+      * constructor. constructor.
+        eapply Forall2_Forall_r in H; first exact H.
+        apply Forall_forall.
+        intros τ Hτ ρ H'.
+        inversion H'. inversion H1.
+        assumption.
+      * eapply Forall2_Forall_l in H; first exact H.
+        apply Forall_forall.
+        intros ρ Hρ τ [Hk Ht].
+        assumption.
+    + constructor. constructor.
+      eapply Forall2_Forall_r in H; first exact H.
+      apply Forall_forall.
+      intros τ Hτ ρ H'.
+      inversion H'. inversion H1.
+      assumption.
+  - split.
+    + constructor.
+      * constructor.
+        -- constructor.
+        -- assumption.
+      * eapply Forall2_Forall_l in H0; first exact H0.
+        apply Forall_forall.
+        intros ζ Hζ τ [Hk Ht].
+        assumption.
+    + constructor.
+      * constructor.
+      * assumption.
+  - split.
+    + constructor.
+      * constructor.
+        -- constructor. constructor.
+           eapply Forall2_Forall_r in H0; first exact H0.
+           apply Forall_forall.
+           intros τ Hτ σ H'.
+           inversion H'. inversion H2. inversion H9.
+           assumption.
+        -- assumption.
+      * eapply Forall2_Forall_l in H0; first exact H0.
+        apply Forall_forall.
+        intros σ Hσ τ [Hk Ht].
+        assumption.
+    + constructor.
+      * constructor. constructor.
+        eapply Forall2_Forall_r in H0; first exact H0.
+        apply Forall_forall.
+        intros τ Hτ σ H'.
+        inversion H'. inversion H2. inversion H9.
+        assumption.
+      * assumption.
+  - split.
+    + constructor.
+      * constructor. constructor.
+        eapply Forall2_Forall_r in H; first exact H.
+        apply Forall_forall.
+        intros τ Hτ ρ H'.
+        inversion H'. inversion H1.
+        assumption.
+      * eapply Forall2_Forall_l in H; first exact H.
+        apply Forall_forall.
+        intros ρ Hρ τ [Hk Ht].
+        assumption.
+    + constructor. constructor.
+      eapply Forall2_Forall_r in H; first exact H.
+      apply Forall_forall.
+      intros τ Hτ ρ H'.
+      inversion H'. inversion H1.
+      assumption.
+  - split.
+    + constructor.
+      * constructor.
+        -- constructor.
+        -- assumption.
+      * eapply Forall2_Forall_l in H0; first exact H0.
+        apply Forall_forall.
+        intros ζ Hζ τ [Hk Ht].
+        assumption.
+    + constructor.
+      * constructor.
+      * assumption.
+  - split.
+    + constructor.
+      * constructor.
+        -- constructor. constructor.
+           eapply Forall2_Forall_r in H0; first exact H0.
+           apply Forall_forall.
+           intros τ Hτ σ H'.
+           inversion H'. inversion H2. inversion H9.
+           assumption.
+        -- assumption.
+      * eapply Forall2_Forall_l in H0; first exact H0.
+        apply Forall_forall.
+        intros σ Hσ τ [Hk Ht].
+        assumption.
+    + constructor.
+      * constructor. constructor.
+        eapply Forall2_Forall_r in H0; first exact H0.
+        apply Forall_forall.
+        intros τ Hτ σ H'.
+        inversion H'. inversion H2. inversion H9.
+        assumption.
+      * assumption.
+  - split.
+    + constructor.
+      * repeat constructor.
+      * inversion IHhas_kind. inversion H0. assumption.
+      * destruct IHhas_kind.
+        assumption.
+    + repeat constructor.
+  - split.
+    + constructor.
+      * repeat constructor.
+      * constructor.
+      * destruct IHhas_kind.
+        assumption.
+    + repeat constructor.
+  - split.
+    + constructor.
+      * repeat constructor.
+      * constructor.
+      * destruct IHhas_kind. assumption.
+    + repeat constructor.
+  - split.
+    + constructor.
+      * repeat constructor.
+      * destruct IHhas_kind. assumption.
+    + repeat constructor.
+  - split.
+    + constructor.
+      * repeat constructor.
+      * assumption.
+    + repeat constructor.
+  - split.
+    + constructor.
+      * constructor. assumption.
+      * assumption.
+      * destruct IHhas_kind. assumption.
+    + constructor. assumption.
+  - split.
+    + constructor.
+      * constructor.
+        -- constructor. assumption.
+        -- inversion IHhas_kind. inversion H1. assumption.
+      * assumption.
+      * destruct IHhas_kind. assumption.
+    + constructor.
+      * constructor. assumption.
+      * inversion IHhas_kind. inversion H1. assumption.
+  - split.
+    + constructor.
+      * constructor.
+        -- constructor. constructor.
+           inversion IHhas_kind. inversion H1. assumption.
+        -- assumption.
+      * destruct IHhas_kind. assumption.
+    + constructor.
+      * constructor. constructor.
+        inversion IHhas_kind.
+        inversion H1. assumption.
+      * assumption.
+  - split.
+    + constructor.
+      * inversion IHhas_kind. simpl in H0. assumption.
+      * inversion IHhas_kind. subst τ0. assumption.
+    + inversion IHhas_kind. simpl in H0. assumption.
+  - split.
+    + constructor.
+      * assumption.
+      * destruct IHhas_kind. assumption.
+    + assumption.
+  - split.
+    + constructor.
+      * assumption.
+      * destruct IHhas_kind. assumption.
+    + assumption.
+  - split.
+    + constructor.
+      * assumption.
+      * destruct IHhas_kind. assumption.
+    + assumption.
+  - split.
+    + constructor.
+      * assumption.
+      * assumption.
+      * destruct IHhas_kind. assumption.
+    + assumption.
+Qed.
